secure_api/prf/Crypto.Symmetric.PRF.fst
@@ -303,7 +303,7 @@ val prf_mac:
       HS.modifies_ref t.mac_rgn TSet.empty h0 h1 )))
 
 
-#reset-options "--z3rlimit 100"
+#reset-options "--z3rlimit 1000 --max_fuel 0 --max_ifuel 0"
 
 let prf_mac i t k_0 x =
   Buffer.recall t.key;
